tutorial/lithium/class_instances.v
@@ -1,0 +1,65 @@
+From lithium.tutorial Require Import notation tactics.
+
+(* This file is a version of proofmode.v from simp-lang:
+   https://github.com/tchajed/iris-simp-lang/blob/main/src/class_instances.v *)
+
+Global Instance into_val_val v : IntoVal (Val v) v.
+Proof. done. Qed.
+Global Instance as_val_val v : AsVal (Val v).
+Proof. by eexists. Qed.
+
+(** * Instances of the [PureExec] class *)
+(** The behavior of the various [wp_] tactics with regard to lambda differs in
+the following way:
+
+- [wp_pures] does *not* reduce lambdas/recs that are hidden behind a definition.
+- [wp_rec] and [wp_lam] reduce lambdas/recs that are hidden behind a definition.
+
+To realize this behavior, we define the class [AsRecV v f x erec], which takes a
+value [v] as its input, and turns it into a [RecV f x erec] via the instance
+[AsRecV_recv : AsRecV (RecV f x e) f x e]. We register this instance via
+[Hint Extern] so that it is only used if [v] is syntactically a lambda/rec, and
+not if [v] contains a lambda/rec that is hidden behind a definition.
+
+To make sure that [wp_rec] and [wp_lam] do reduce lambdas/recs that are hidden
+behind a definition, we activate [AsRecV_recv] by hand in these tactics. *)
+Class AsRecV (v : val) (f x : binder) (erec : expr) :=
+  as_recv : v = RecV f x erec.
+Global Hint Mode AsRecV ! - - - : typeclass_instances.
+Definition AsRecV_recv f x e : AsRecV (RecV f x e) f x e := eq_refl.
+Global Hint Extern 0 (AsRecV (RecV _ _ _) _ _ _) =>
+  apply AsRecV_recv : typeclass_instances.
+
+Section pure_exec.
+  Local Ltac solve_exec_safe := intros; subst; do 3 eexists; econstructor; eauto.
+  Local Ltac solve_exec_puredet := simpl; intros; by inv_head_step.
+  Local Ltac solve_pure_exec :=
+    subst; intros ?; apply nsteps_once, pure_head_step_pure_step;
+      constructor; [solve_exec_safe | solve_exec_puredet].
+
+  Global Instance pure_recc f x (erec : expr) :
+    PureExec True 1 (Rec f x erec) (Val $ RecV f x erec).
+  Proof. solve_pure_exec. Qed.
+  Global Instance pure_beta f x (erec : expr) (v1 v2 : val) `{!AsRecV v1 f x erec} :
+    PureExec True 1 (App (Val v1) (Val v2)) (subst' x v2 (subst' f v1 erec)).
+  Proof. unfold AsRecV in *. solve_pure_exec. Qed.
+
+  Global Instance pure_unop op v v' :
+    PureExec (un_op_eval op v = Some v') 1 (UnOp op (Val v)) (Val v').
+  Proof. solve_pure_exec. Qed.
+
+  Global Instance pure_binop op v1 v2 v' :
+    PureExec (bin_op_eval op v1 v2 = Some v') 1 (BinOp op (Val v1) (Val v2)) (Val v') | 10.
+  Proof. solve_pure_exec. Qed.
+
+  Global Instance pure_if_true e1 e2 :
+    PureExec True 1 (If (Val $ LitV $ LitBool true) e1 e2) e1.
+  Proof. solve_pure_exec. Qed.
+  Global Instance pure_if_false e1 e2 :
+    PureExec True 1 (If (Val $ LitV $ LitBool false) e1 e2) e2.
+  Proof. solve_pure_exec. Qed.
+
+  Global Instance pure_assert :
+    PureExec True 1 (Assert (Val $ LitV $ LitBool true)) (Val $ LitV $ LitInt 0).
+  Proof. solve_pure_exec. Qed.
+End pure_exec.
