tutorial/lithium/proofmode.v
@@ -1,0 +1,142 @@
+From iris.proofmode Require Import coq_tactics reduction.
+From iris.proofmode Require Import tactics.
+From iris.program_logic Require Import atomic.
+From lithium.tutorial Require Import tactics class_instances primitive_laws notation.
+
+(* This file is a version of proofmode.v from simp-lang:
+   https://github.com/tchajed/iris-simp-lang/blob/main/src/proofmode.v *)
+
+Lemma tac_wp_expr_eval `{!tutorialGS Σ} Δ s E Φ e e' :
+  (∀ (e'':=e'), e = e'') →
+  envs_entails Δ (WP e' @ s; E {{ Φ }}) → envs_entails Δ (WP e @ s; E {{ Φ }}).
+Proof. by intros ->. Qed.
+
+Tactic Notation "wp_expr_eval" tactic3(t) :=
+  iStartProof;
+  lazymatch goal with
+  | |- envs_entails _ (wp ?s ?E ?e ?Q) =>
+    notypeclasses refine (tac_wp_expr_eval _ _ _ _ e _ _ _);
+      [let x := fresh in intros x; t; unfold x; notypeclasses refine eq_refl|]
+  | _ => fail "wp_expr_eval: not a 'wp'"
+  end.
+Ltac wp_expr_simpl := wp_expr_eval simpl.
+
+Lemma tac_wp_pure `{!tutorialGS Σ} Δ Δ' s E K e1 e2 φ n Φ :
+  PureExec φ n e1 e2 →
+  φ →
+  MaybeIntoLaterNEnvs n Δ Δ' →
+  envs_entails Δ' (WP (fill K e2) @ s; E {{ Φ }}) →
+  envs_entails Δ (WP (fill K e1) @ s; E {{ Φ }}).
+Proof.
+  rewrite envs_entails_unseal=> ??? HΔ'. rewrite into_laterN_env_sound /=.
+  (* We want [pure_exec_fill] to be available to TC search locally. *)
+  pose proof @pure_exec_fill.
+  rewrite HΔ' -lifting.wp_pure_step_later //.
+  iIntros "Hwp !> _" => //.
+Qed.
+
+Lemma tac_wp_value_nofupd `{!tutorialGS Σ} Δ s E Φ v :
+  envs_entails Δ (Φ v) → envs_entails Δ (WP (Val v) @ s; E {{ Φ }}).
+Proof. rewrite envs_entails_unseal=> ->. by apply wp_value. Qed.
+
+Lemma tac_wp_value `{!tutorialGS Σ} Δ s E (Φ : val → iPropI Σ) v :
+  envs_entails Δ (|={E}=> Φ v) → envs_entails Δ (WP (Val v) @ s; E {{ Φ }}).
+Proof. rewrite envs_entails_unseal=> ->. by rewrite wp_value_fupd. Qed.
+
+(** Simplify the goal if it is [WP] of a value.
+  If the postcondition already allows a fupd, do not add a second one.
+  But otherwise, *do* add a fupd. This ensures that all the lemmas applied
+  here are bidirectional, so we never will make a goal unprovable. *)
+Ltac wp_value_head :=
+  lazymatch goal with
+  | |- envs_entails _ (wp ?s ?E (Val _) (λ _, fupd ?E _ _)) =>
+      eapply tac_wp_value_nofupd
+  | |- envs_entails _ (wp ?s ?E (Val _) (λ _, wp _ ?E _ _)) =>
+      eapply tac_wp_value_nofupd
+  | |- envs_entails _ (wp ?s ?E (Val _) _) =>
+      eapply tac_wp_value
+  end.
+
+Ltac wp_finish :=
+  wp_expr_simpl;      (* simplify occurences of subst/fill *)
+  try wp_value_head;  (* in case we have reached a value, get rid of the WP *)
+  pm_prettify.        (* prettify ▷s caused by [MaybeIntoLaterNEnvs] and
+                         λs caused by wp_value *)
+
+(** The argument [efoc] can be used to specify the construct that should be
+reduced. For example, you can write [wp_pure (EIf _ _ _)], which will search
+for an [EIf _ _ _] in the expression, and reduce it.
+
+The use of [open_constr] in this tactic is essential. It will convert all holes
+(i.e. [_]s) into evars, that later get unified when an occurences is found
+(see [unify e' efoc] in the code below). *)
+Tactic Notation "wp_pure" open_constr(efoc) :=
+  iStartProof;
+  lazymatch goal with
+  | |- envs_entails _ (wp ?s ?E ?e ?Q) =>
+    let e := eval simpl in e in
+    reshape_expr e ltac:(fun K e' =>
+      unify e' efoc;
+      eapply (tac_wp_pure _ _ _ _ K e');
+      [tc_solve                       (* PureExec *)
+      |try fast_done
+      |tc_solve                       (* IntoLaters *)
+      |wp_finish                      (* new goal *)
+      ])
+    || fail "wp_pure: cannot find" efoc "in" e "or" efoc "is not a redex"
+  | _ => fail "wp_pure: not a 'wp'"
+  end.
+
+Ltac wp_pures :=
+  iStartProof;
+  first [ (* The `;[]` makes sure that no side-condition magically spawns. *)
+          progress repeat (wp_pure _; [])
+        | wp_finish (* In case wp_pure never ran, make sure we do the usual cleanup. *)
+        ].
+
+(** Unlike [wp_pures], the tactics [wp_rec] and [wp_lam] should also reduce
+lambdas/recs that are hidden behind a definition, i.e. they should use
+[AsRecV_recv] as a proper instance instead of a [Hint Extern].
+
+We achieve this by putting [AsRecV_recv] in the current environment so that it
+can be used as an instance by the typeclass resolution system. We then perform
+the reduction, and finally we clear this new hypothesis. *)
+Tactic Notation "wp_rec" :=
+  let H := fresh in
+  pose proof (H := AsRecV_recv);
+  wp_pure (App _ _);
+  clear H.
+
+Tactic Notation "wp_if" := wp_pure (If _ _ _).
+Tactic Notation "wp_if_true" := wp_pure (If (LitV (LitBool true)) _ _).
+Tactic Notation "wp_if_false" := wp_pure (If (LitV (LitBool false)) _ _).
+Tactic Notation "wp_unop" := wp_pure (UnOp _ _).
+Tactic Notation "wp_binop" := wp_pure (BinOp _ _ _).
+Tactic Notation "wp_op" := wp_unop || wp_binop.
+Tactic Notation "wp_lam" := wp_rec.
+Tactic Notation "wp_let" := wp_pure (Rec BAnon (BNamed _) _); wp_lam.
+Tactic Notation "wp_seq" := wp_pure (Rec BAnon BAnon _); wp_lam.
+Tactic Notation "wp_proj" := wp_pure (Fst _) || wp_pure (Snd _).
+Tactic Notation "wp_pair" := wp_pure (Pair _ _).
+Tactic Notation "wp_closure" := wp_pure (Rec _ _ _).
+
+Lemma tac_wp_bind `{!tutorialGS Σ} K Δ s E Φ e f :
+  f = (λ e, fill K e) → (* as an eta expanded hypothesis so that we can `simpl` it *)
+  envs_entails Δ (WP e @ s; E {{ v, WP f (Val v) @ s; E {{ Φ }} }})%I →
+  envs_entails Δ (WP fill K e @ s; E {{ Φ }}).
+Proof. rewrite envs_entails_unseal=> -> ->. by apply: wp_bind. Qed.
+
+Ltac wp_bind_core K :=
+  lazymatch eval hnf in K with
+  | [] => idtac
+  | _ => eapply (tac_wp_bind K); [simpl; reflexivity|reduction.pm_prettify]
+  end.
+
+Tactic Notation "wp_bind" open_constr(efoc) :=
+  iStartProof;
+  lazymatch goal with
+  | |- envs_entails _ (wp ?s ?E ?e ?Q) =>
+    first [ reshape_expr e ltac:(fun K e' => unify e' efoc; wp_bind_core K)
+          | fail 1 "wp_bind: cannot find" efoc "in" e ]
+  | _ => fail "wp_bind: not a 'wp'"
+  end.
